theories/typing.v
@@ -15,7 +15,7 @@ Section Typing.
 
   (* Helping the inference with this notation that hides Δ *)
   Local Notation "Γ ⊢ s <: t" := (@subtype _ Γ Plain s t) (at level 70, s at next level, no associativity).
-  Local Notation "Γ ⊢ lty <:< rty" := (@lty_sub _ Γ lty rty) (lty at next level, at level 70, no associativity).
+  Local Notation "Γ ⊢ s <D: t" := (@subtype _ Γ Aware s t) (at level 70, s at next level, no associativity).
 
   (* At class + substitution is `ok` w.r.t. to a set of constraints `Γ` if
    * - all the types in the substitution are ok
@@ -29,7 +29,7 @@ Section Typing.
     | OkClass t σ def:
         (∀ i ty, σ !! i = Some ty → ok_ty Γ ty) →
         Δ !! t = Some def →
-        (∀ i c, def.(constraints) !! i = Some c → Γ ⊢ (subst_ty σ c.1) <: (subst_ty σ c.2)) →
+        (∀ i c, def.(constraints) !! i = Some c → Γ ⊢ (subst_ty σ c.1) <D: (subst_ty σ c.2)) →
         ok_ty Γ (ClassT t σ)
     | OkNull: ok_ty Γ NullT
     | OkNonNull: ok_ty Γ NonNullT
@@ -44,11 +44,11 @@ Section Typing.
   Lemma ok_ty_constraint_elim_ G T:
     ok_ty G T →
     ∀ Γ Γ', G = Γ ++ Γ' →
-    (∀ i c, Γ' !! i = Some c → Γ ⊢ c.1 <: c.2) →
+    (∀ i c, Γ' !! i = Some c → Γ ⊢ c.1 <D: c.2) →
     ok_ty Γ T.
   Proof.
     induction 1 as [ | | | | t σ def hσ hi hdef hconstr
-    | | | s t hs hi ht hit | s t hs hi ht hit | n | t | | ] => Γ Γ' heq hΓ; subst; try by constructor.
+    | | | s t hs hi ht hit | s t hs hi ht hit | | | | ] => Γ Γ' heq hΓ; subst; try by constructor.
     - apply OkClass with def => //.
       + move => i ty h; by eapply hi.
       + move => i c h.
@@ -59,7 +59,7 @@ Section Typing.
 
   Lemma ok_ty_constraint_elim Γ Γ' T:
     ok_ty (Γ ++ Γ') T →
-    (∀ i c, Γ' !! i = Some c → Γ ⊢ c.1 <: c.2) →
+    (∀ i c, Γ' !! i = Some c → Γ ⊢ c.1 <D: c.2) →
     ok_ty Γ T.
   Proof. intros; by eapply ok_ty_constraint_elim_. Qed.
 
@@ -169,7 +169,7 @@ Section Typing.
   Lemma ok_ty_trans Γ ty:
     ok_ty Γ ty →
     ∀ Γ',
-    (∀ i c, Γ !! i = Some c → Γ' ⊢ c.1 <: c.2) →
+    (∀ i c, Γ !! i = Some c → Γ' ⊢ c.1 <D: c.2) →
     ok_ty Γ' ty.
   Proof.
     induction 1 as [ | | | | t σ def hσ hi hdef hconstr
@@ -296,59 +296,59 @@ Section Typing.
     end
   .
 
-  Inductive expr_has_ty Γ (lty : local_tys) :
-    expr → lang_ty → Prop :=
-    | IntTy : ∀ z, expr_has_ty Γ lty (IntE z) IntT
-    | BoolTy: ∀ b, expr_has_ty Γ lty (BoolE b) BoolT
-    | NullTy: expr_has_ty Γ lty NullE NullT
-    | BinOpIntTy: ∀ op e1 e2,
+  Inductive expr_has_ty Γ (lty : local_tys):
+    subtype_kind → expr → lang_ty → Prop :=
+    | IntTy : ∀ kd z, expr_has_ty Γ lty kd (IntE z) IntT
+    | BoolTy: ∀ kd b, expr_has_ty Γ lty kd (BoolE b) BoolT
+    | NullTy kd: expr_has_ty Γ lty kd NullE NullT
+    | BinOpIntTy: ∀ kd op e1 e2,
         is_bool_op op = false →
-        expr_has_ty Γ lty e1 IntT →
-        expr_has_ty Γ lty e2 IntT →
-        expr_has_ty Γ lty (BinOpE op e1 e2) IntT
-    | BinOpBoolTy: ∀ op e1 e2,
+        expr_has_ty Γ lty kd e1 IntT →
+        expr_has_ty Γ lty kd e2 IntT →
+        expr_has_ty Γ lty kd (BinOpE op e1 e2) IntT
+    | BinOpBoolTy: ∀ kd op e1 e2,
         is_bool_op op = true →
-        expr_has_ty Γ lty e1 IntT →
-        expr_has_ty Γ lty e2 IntT →
-        expr_has_ty Γ lty (BinOpE op e1 e2) BoolT
-    | EqBoolTy: ∀ e1 e2,
-        expr_has_ty Γ lty e1 BoolT →
-        expr_has_ty Γ lty e2 BoolT →
-        expr_has_ty Γ lty (BinOpE EqO e1 e2) BoolT
-    | UniOpTy: ∀ e,
-        expr_has_ty Γ lty e BoolT →
-        expr_has_ty Γ lty (UniOpE NotO e) BoolT
-    | GenTy: ∀ v ty,
+        expr_has_ty Γ lty kd e1 IntT →
+        expr_has_ty Γ lty kd e2 IntT →
+        expr_has_ty Γ lty kd (BinOpE op e1 e2) BoolT
+    | EqBoolTy: ∀ kd e1 e2,
+        expr_has_ty Γ lty kd e1 BoolT →
+        expr_has_ty Γ lty kd e2 BoolT →
+        expr_has_ty Γ lty kd (BinOpE EqO e1 e2) BoolT
+    | UniOpTy: ∀ kd e,
+        expr_has_ty Γ lty kd e BoolT →
+        expr_has_ty Γ lty kd (UniOpE NotO e) BoolT
+    | GenTy: ∀ kd v ty,
         lty.(ctxt) !! v = Some ty →
-        expr_has_ty Γ lty (VarE v) ty
-    | ThisTy : expr_has_ty Γ lty ThisE (this_type lty)
-    | ESubTy: ∀ e s t,
-        expr_has_ty Γ lty e s →
+        expr_has_ty Γ lty kd (VarE v) ty
+    | ThisTy kd: expr_has_ty Γ lty kd ThisE (this_type lty)
+    | ESubTy: ∀ kd e s t,
+        expr_has_ty Γ lty kd e s →
         wf_ty t →
         ok_ty Γ t →
-        Γ ⊢ s <: t →
-        expr_has_ty Γ lty e t
-    (* SD.V1 we don't distinguish between plain subtyping vs
-       dynamic aware subtyping. But we do add the new
-       rule in preparation for that.
+        subtype Γ kd s t →
+        expr_has_ty Γ lty kd e t
+    (* SD.V2 we don't distinguish between plain subtyping vs
+       dynamic aware subtyping. Yet, we'll turn the switch
+       in the next commit, once all judgments are "kind" aware.
      *)
-    | UpcastTy: ∀ e s t,
-        expr_has_ty Γ lty e s →
+    | UpcastTy: ∀ kd e s t,
+        expr_has_ty Γ lty kd e s →
         wf_ty t →
         ok_ty Γ t →
-        Γ ⊢ s <: t →
-        expr_has_ty Γ lty (UpcastE e t) t
+        subtype Γ kd s t →
+        expr_has_ty Γ lty kd (UpcastE e t) t
   .
 
-  Lemma expr_has_ty_constraint_elim_ G lty e ty:
-    expr_has_ty G lty e ty →
+  Lemma expr_has_ty_constraint_elim_ G kd lty e ty:
+    expr_has_ty G lty kd e ty →
     ∀ Γ Γ', G = Γ ++ Γ' →
-    (∀ i c, Γ' !! i = Some c → Γ ⊢ c.1 <: c.2) →
-    expr_has_ty Γ lty e ty.
+    (∀ i c, Γ' !! i = Some c → Γ ⊢ c.1 <D: c.2) →
+    expr_has_ty Γ lty kd e ty.
   Proof.
-    induction 1 as [ z | b | | op e1 e2 hop h1 hi1 h2 hi2 |
-      op e1 e2 hop h1 hi1 h2 hi2 | e1 e2 h1 hi1 h2 hi2 | e h hi | v ty h | |
-      e s t h hi hok hsub | e s t h hi hok hsub] => Γ Γ' heq hΓ; subst; try (by constructor).
+    induction 1 as [ | | | kd op e1 e2 hop h1 hi1 h2 hi2 |
+      kd op e1 e2 hop h1 hi1 h2 hi2 | kd e1 e2 h1 hi1 h2 hi2 | kd e h hi | kd v ty h | |
+      kd e s t h hi hok hsub | kd e s t h hi hok hsub] => Γ Γ' heq hΓ; subst; try (by constructor).
     - constructor; by eauto.
     - constructor; by eauto.
     - constructor; by eauto.
@@ -365,24 +365,24 @@ Section Typing.
       + by eapply subtype_constraint_elim.
   Qed.
 
-  Lemma expr_has_ty_constraint_elim Γ Γ' lty e ty:
-    expr_has_ty (Γ ++ Γ') lty e ty →
-    (∀ i c, Γ' !! i = Some c → Γ ⊢ c.1 <: c.2) →
-    expr_has_ty Γ lty e ty.
+  Lemma expr_has_ty_constraint_elim Γ Γ' kd lty e ty:
+    expr_has_ty (Γ ++ Γ') lty kd e ty →
+    (∀ i c, Γ' !! i = Some c → Γ ⊢ c.1 <D: c.2) →
+    expr_has_ty Γ lty kd e ty.
   Proof. intros; by eapply expr_has_ty_constraint_elim_. Qed.
 
-  Lemma expr_has_ty_subst Γ' Γ σ lty e ty:
+  Lemma expr_has_ty_subst Γ' Γ kd σ lty e ty:
     map_Forall (λ _ : string, wf_cdef_parent Δ) Δ →
     map_Forall (λ _ : string, wf_cdef_constraints_bounded) Δ →
     Forall wf_ty σ →
     Forall (ok_ty Γ') σ →
-    expr_has_ty Γ lty e ty →
-    expr_has_ty (Γ' ++ (subst_constraints σ Γ)) (subst_lty σ lty) (subst_expr σ e) (subst_ty σ ty).
+    expr_has_ty Γ lty kd e ty →
+    expr_has_ty (Γ' ++ (subst_constraints σ Γ)) (subst_lty σ lty) kd (subst_expr σ e) (subst_ty σ ty).
   Proof.
     move => hp hb hσwf hσok.
-    induction 1 as [ z | b | | op e1 e2 hop h1 hi1 h2 hi2 |
-      op e1 e2 hop h1 hi1 h2 hi2 | e1 e2 h1 hi1 h2 hi2 | e h hi |
-      v ty h | | e s t h hi hok hsub | e s t h hi hok hsub ] => //=; try (by constructor).
+    induction 1 as [ | | | kd op e1 e2 hop h1 hi1 h2 hi2 |
+      kd op e1 e2 hop h1 hi1 h2 hi2 | kd e1 e2 h1 hi1 h2 hi2 | kd e h hi |
+      kd v ty h | | kd e s t h hi hok hsub | kd e s t h hi hok hsub ] => //=; try (econstructor; by eauto).
     - constructor.
       rewrite /subst_lty /=.
       by rewrite lookup_fmap h.
@@ -398,12 +398,12 @@ Section Typing.
         by set_solver.
   Qed.
 
-  Lemma expr_has_ty_weaken Γ lty e ty:
-    expr_has_ty Γ lty e ty → ∀ Γ', Γ ⊆ Γ' → expr_has_ty Γ' lty e ty.
+  Lemma expr_has_ty_weaken Γ lty kd e ty:
+    expr_has_ty Γ lty kd e ty → ∀ Γ', Γ ⊆ Γ' → expr_has_ty Γ' lty kd e ty.
   Proof.
-    induction 1 as [ z | b | | op e1 e2 hop h1 hi1 h2 hi2 |
-      op e1 e2 hop h1 hi1 h2 hi2 | e1 e2 h1 hi1 h2 hi2 | e h hi |
-      v ty h | | e s t h hi hok hsub | e s t h hi hok hsub ] => Γ' hincl;
+    induction 1 as [ | | | kd op e1 e2 hop h1 hi1 h2 hi2 |
+      kd op e1 e2 hop h1 hi1 h2 hi2 | kd e1 e2 h1 hi1 h2 hi2 | kd e h hi |
+      kd v ty h | | kd e s t h hi hok hsub | kd e s t h hi hok hsub ] => Γ' hincl;
           try (econstructor; by eauto).
      - eapply ESubTy.
        + by eapply hi.
@@ -454,15 +454,15 @@ Section Typing.
       by apply hl in hk.
   Qed.
 
-  Lemma expr_has_ty_wf Γ lty e ty:
+  Lemma expr_has_ty_wf Γ kd lty e ty:
     wf_lty lty →
-    expr_has_ty Γ lty e ty →
+    expr_has_ty Γ lty kd e ty →
     wf_ty ty.
   Proof.
     move => hwf.
-    induction 1 as [ z | b | | op e1 e2 hop h1 hi1 h2 hi2 |
-      op e1 e2 hop h1 hi1 h2 hi2 | e1 e2 h1 hi1 h2 hi2 | e h hi |
-      v ty h | | e s t h hi hsub | e s t h hi hsub] => //=; try (by constructor).
+    induction 1 as [ | | | kd op e1 e2 hop h1 hi1 h2 hi2 |
+      kd op e1 e2 hop h1 hi1 h2 hi2 | kd e1 e2 h1 hi1 h2 hi2 | kd e h hi |
+      kd v ty h | | kd e s t h hi hsub | kd e s t h hi hsub] => //=; try (by constructor).
     - by apply hwf in h.
     - by apply hwf.
   Qed.
@@ -472,53 +472,53 @@ Section Typing.
     map_Forall (λ _, ok_ty Γ) lty.(ctxt)
   .
 
-  Lemma expr_has_ty_ok Γ lty e ty:
+  Lemma expr_has_ty_ok Γ lty kd e ty:
     ok_lty Γ lty →
-    expr_has_ty Γ lty e ty →
+    expr_has_ty Γ lty kd e ty →
     ok_ty Γ ty.
   Proof.
     move => hok.
-    induction 1 as [ z | b | | op e1 e2 hop h1 hi1 h2 hi2 |
-      op e1 e2 hop h1 hi1 h2 hi2 | e1 e2 h1 hi1 h2 hi2 | e h hi |
-      v ty h | | e s t h hi hsub | e s t h hi hsub] => //=; try (by constructor).
+    induction 1 as [ | | | kd op e1 e2 hop h1 hi1 h2 hi2 |
+      kd op e1 e2 hop h1 hi1 h2 hi2 | kd e1 e2 h1 hi1 h2 hi2 | kd e h hi |
+      kd v ty h | | kd e s t h hi hsub | kd e s t h hi hsub] => //=; try (by constructor).
     - by apply hok in h.
     - by apply hok.
   Qed.
 
   (* continuation-based typing for commands *)
-  Inductive cmd_has_ty Γ : local_tys → cmd → local_tys → Prop :=
-    | SkipTy: ∀ lty, cmd_has_ty Γ lty SkipC lty
-    | SeqTy: ∀ lty1 lty2 lty3 fstc sndc,
-        cmd_has_ty Γ lty1 fstc lty2 →
-        cmd_has_ty Γ lty2 sndc lty3 →
-        cmd_has_ty Γ lty1 (SeqC fstc sndc) lty3
-    | LetTy: ∀ lty lhs e ty,
-        expr_has_ty Γ lty e ty →
-        cmd_has_ty Γ lty (LetC lhs e) (<[lhs := ty]>lty)
-    | IfTy: ∀ lty1 lty2 cond thn els,
-        expr_has_ty Γ lty1 cond BoolT →
-        cmd_has_ty Γ lty1 thn lty2 →
-        cmd_has_ty Γ lty1 els lty2 →
-        cmd_has_ty Γ lty1 (IfC cond thn els) lty2
-    | GetPrivTy: ∀ lty lhs t σ name fty,
+  Inductive cmd_has_ty Γ : subtype_kind → local_tys → cmd → local_tys → Prop :=
+    | SkipTy: ∀ lty kd, cmd_has_ty Γ kd lty SkipC lty
+    | SeqTy: ∀ kd lty1 lty2 lty3 fstc sndc,
+        cmd_has_ty Γ kd lty1 fstc lty2 →
+        cmd_has_ty Γ kd lty2 sndc lty3 →
+        cmd_has_ty Γ kd lty1 (SeqC fstc sndc) lty3
+    | LetTy: ∀ kd lty lhs e ty,
+        expr_has_ty Γ lty kd e ty →
+        cmd_has_ty Γ kd lty (LetC lhs e) (<[lhs := ty]>lty)
+    | IfTy: ∀ kd lty1 lty2 cond thn els,
+        expr_has_ty Γ lty1 kd cond BoolT →
+        cmd_has_ty Γ kd lty1 thn lty2 →
+        cmd_has_ty Γ kd lty1 els lty2 →
+        cmd_has_ty Γ kd lty1 (IfC cond thn els) lty2
+    | GetPrivTy: ∀ kd lty lhs t σ name fty,
         type_of_this lty = (t, σ) →
         has_field name t Private fty t →
-        cmd_has_ty Γ lty (GetC lhs ThisE name) (<[lhs := subst_ty σ fty]>lty)
-    | GetPubTy: ∀ lty lhs recv t σ name fty orig,
-        expr_has_ty Γ lty recv (ClassT t σ) →
+        cmd_has_ty Γ kd lty (GetC lhs ThisE name) (<[lhs := subst_ty σ fty]>lty)
+    | GetPubTy: ∀ kd lty lhs recv t σ name fty orig,
+        expr_has_ty Γ lty kd recv (ClassT t σ) →
         has_field name t Public fty orig →
-        cmd_has_ty Γ lty (GetC lhs recv name) (<[lhs := subst_ty σ fty]>lty)
-    | SetPrivTy: ∀ lty fld rhs fty t σ,
+        cmd_has_ty Γ kd lty (GetC lhs recv name) (<[lhs := subst_ty σ fty]>lty)
+    | SetPrivTy: ∀ kd lty fld rhs fty t σ,
         type_of_this lty = (t, σ) →
         has_field fld t Private fty t →
-        expr_has_ty Γ lty rhs (subst_ty σ fty) →
-        cmd_has_ty Γ lty (SetC ThisE fld rhs) lty
-    | SetPubTy: ∀ lty recv fld rhs fty orig t σ,
-        expr_has_ty Γ lty recv (ClassT t σ) →
+        expr_has_ty Γ lty kd rhs (subst_ty σ fty) →
+        cmd_has_ty Γ kd lty (SetC ThisE fld rhs) lty
+    | SetPubTy: ∀ kd lty recv fld rhs fty orig t σ,
+        expr_has_ty Γ lty kd recv (ClassT t σ) →
         has_field fld t Public fty orig →
-        expr_has_ty Γ lty rhs (subst_ty σ fty) →
-        cmd_has_ty Γ lty (SetC recv fld rhs) lty
-    | NewTy: ∀ lty lhs t targs args fields,
+        expr_has_ty Γ lty kd rhs (subst_ty σ fty) →
+        cmd_has_ty Γ kd lty (SetC recv fld rhs) lty
+    | NewTy: ∀ kd lty lhs t targs args fields,
         wf_ty (ClassT t targs) →
         ok_ty Γ (ClassT t targs) →
         has_fields t fields →
@@ -526,90 +526,90 @@ Section Typing.
         (∀ f fty arg,
         fields !! f = Some fty →
         args !! f = Some arg →
-        expr_has_ty Γ lty arg (subst_ty targs fty.1.2)) →
-        cmd_has_ty Γ lty (NewC lhs t targs args) (<[lhs := ClassT t targs]>lty)
-    | CallTy: ∀ lty lhs recv t targs name orig mdef args,
-        expr_has_ty Γ lty recv (ClassT t targs) →
+        expr_has_ty Γ lty kd arg (subst_ty targs fty.1.2)) →
+        cmd_has_ty Γ kd lty (NewC lhs t targs args) (<[lhs := ClassT t targs]>lty)
+    | CallTy: ∀ kd lty lhs recv t targs name orig mdef args,
+        expr_has_ty Γ lty kd recv (ClassT t targs) →
         has_method name t orig mdef →
         dom mdef.(methodargs) = dom args →
         (∀ x ty arg,
         mdef.(methodargs) !! x = Some ty →
         args !! x = Some arg →
-        expr_has_ty Γ lty arg (subst_ty targs ty)) →
-        cmd_has_ty Γ lty (CallC lhs recv name args) (<[lhs := subst_ty targs mdef.(methodrettype)]>lty)
-    | SubTy: ∀ lty c rty rty',
-        Γ ⊢ rty' <:< rty →
-        cmd_has_ty Γ lty c rty' →
-        cmd_has_ty Γ lty c rty
-    | TagCheckTy lty rty v tv t cmd :
+        expr_has_ty Γ lty kd arg (subst_ty targs ty)) →
+        cmd_has_ty Γ kd lty (CallC lhs recv name args) (<[lhs := subst_ty targs mdef.(methodrettype)]>lty)
+    | SubTy: ∀ kd lty c rty rty',
+        lty_sub Γ kd rty' rty →
+        cmd_has_ty Γ kd lty c rty' →
+        cmd_has_ty Γ kd lty c rty
+    | TagCheckTy kd lty rty v tv t cmd :
         lty.(ctxt) !! v = Some tv →
-        Γ ⊢ lty <:< rty →
-        cmd_has_ty Γ (<[v:=InterT tv (ExT t)]> lty) cmd rty →
-        cmd_has_ty Γ lty (RuntimeCheckC v (RCTag t) cmd) rty
-    | IntCheckTy lty rty v tv cmd :
+        lty_sub Γ kd lty rty →
+        cmd_has_ty Γ kd (<[v:=InterT tv (ExT t)]> lty) cmd rty →
+        cmd_has_ty Γ kd lty (RuntimeCheckC v (RCTag t) cmd) rty
+    | IntCheckTy kd lty rty v tv cmd :
         lty.(ctxt) !! v = Some tv →
-        Γ ⊢ lty <:< rty →
-        cmd_has_ty Γ (<[v:=InterT tv IntT]> lty) cmd rty →
-        cmd_has_ty Γ lty (RuntimeCheckC v RCInt cmd) rty
-    | BoolCheckTy lty rty v tv cmd :
+        lty_sub Γ kd lty rty →
+        cmd_has_ty Γ kd (<[v:=InterT tv IntT]> lty) cmd rty →
+        cmd_has_ty Γ kd lty (RuntimeCheckC v RCInt cmd) rty
+    | BoolCheckTy kd lty rty v tv cmd :
         lty.(ctxt) !! v = Some tv →
-        Γ ⊢ lty <:< rty →
-        cmd_has_ty Γ (<[v:=InterT tv BoolT]> lty) cmd rty →
-        cmd_has_ty Γ lty (RuntimeCheckC v RCBool cmd) rty
-    | NullCheckTy lty rty v tv cmd :
+        lty_sub Γ kd lty rty →
+        cmd_has_ty Γ kd (<[v:=InterT tv BoolT]> lty) cmd rty →
+        cmd_has_ty Γ kd lty (RuntimeCheckC v RCBool cmd) rty
+    | NullCheckTy kd lty rty v tv cmd :
         lty.(ctxt) !! v = Some tv →
-        Γ ⊢ lty <:< rty →
-        cmd_has_ty Γ (<[v:=InterT tv NullT]> lty) cmd rty →
-        cmd_has_ty Γ lty (RuntimeCheckC v RCNull cmd) rty
-    | NonNullCheckTy lty rty v tv cmd :
+        lty_sub Γ kd lty rty →
+        cmd_has_ty Γ kd (<[v:=InterT tv NullT]> lty) cmd rty →
+        cmd_has_ty Γ kd lty (RuntimeCheckC v RCNull cmd) rty
+    | NonNullCheckTy kd lty rty v tv cmd :
         lty.(ctxt) !! v = Some tv →
-        Γ ⊢ lty <:< rty →
-        cmd_has_ty Γ (<[v:=InterT tv NonNullT]> lty) cmd rty →
-        cmd_has_ty Γ lty (RuntimeCheckC v RCNonNull cmd) rty
+        lty_sub Γ kd lty rty →
+        cmd_has_ty Γ kd (<[v:=InterT tv NonNullT]> lty) cmd rty →
+        cmd_has_ty Γ kd lty (RuntimeCheckC v RCNonNull cmd) rty
     (* Dynamic related typing rules *)
-    | DynIfTy: ∀ lty1 lty2 cond thn els,
-        expr_has_ty Γ lty1 cond DynamicT →
-        cmd_has_ty Γ lty1 thn lty2 →
-        cmd_has_ty Γ lty1 els lty2 →
-        cmd_has_ty Γ lty1 (IfC cond thn els) lty2
-    | DynGetTy : ∀ lty lhs recv name,
-        expr_has_ty Γ lty recv DynamicT →
+    | DynIfTy: ∀ kd lty1 lty2 cond thn els,
+        expr_has_ty Γ lty1 kd cond DynamicT →
+        cmd_has_ty Γ kd lty1 thn lty2 →
+        cmd_has_ty Γ kd lty1 els lty2 →
+        cmd_has_ty Γ kd lty1 (IfC cond thn els) lty2
+    | DynGetTy : ∀ kd lty lhs recv name,
+        expr_has_ty Γ lty kd recv DynamicT →
         (match recv with
          | ThisE => False
          | _ => True
          end
         ) →
-        cmd_has_ty Γ lty (GetC lhs recv name) (<[lhs := DynamicT]>lty)
-    | DynSetTy : ∀ lty recv fld rhs,
-        expr_has_ty Γ lty recv DynamicT →
-        expr_has_ty Γ lty rhs DynamicT →
+        cmd_has_ty Γ kd lty (GetC lhs recv name) (<[lhs := DynamicT]>lty)
+    | DynSetTy : ∀ kd lty recv fld rhs,
+        expr_has_ty Γ lty kd recv DynamicT →
+        expr_has_ty Γ lty kd rhs DynamicT →
         (match recv with
          | ThisE => False
          | _ => True
          end) →
-        cmd_has_ty Γ lty (SetC recv fld rhs) lty
-    | DynCallTy: ∀ lty lhs recv name (args: stringmap expr),
-        expr_has_ty Γ lty recv DynamicT →
+        cmd_has_ty Γ kd lty (SetC recv fld rhs) lty
+    | DynCallTy: ∀ kd lty lhs recv name (args: stringmap expr),
+        expr_has_ty Γ lty kd recv DynamicT →
         (∀ x arg, args !! x = Some arg →
-          expr_has_ty Γ lty arg DynamicT) →
+          expr_has_ty Γ lty kd arg DynamicT) →
         (match recv with
          | ThisE => False
          | _ => True
          end) →
-        cmd_has_ty Γ lty (CallC lhs recv name args) (<[lhs := DynamicT]>lty)
+        cmd_has_ty Γ kd lty (CallC lhs recv name args) (<[lhs := DynamicT]>lty)
   .
 
-  Lemma cmd_has_ty_constraint_weaken Γ lty cmd rty:
-    cmd_has_ty Γ lty cmd rty → ∀ Γ', Γ ⊆ Γ' → cmd_has_ty Γ' lty cmd rty.
+  Lemma cmd_has_ty_constraint_weaken Γ kd lty cmd rty:
+    cmd_has_ty Γ kd lty cmd rty → ∀ Γ', Γ ⊆ Γ' → cmd_has_ty Γ' kd lty cmd rty.
   Proof.
-    induction 1 as [ lty | ????? h1 hi1 h2 hi2 | ???? he |
-      ????? he h1 hi1 h2 hi2 | ?????? he hf | ???????? he hf |
-      ?????? he hf hr | ???????? he hf hr | ?????? ht hok hf hdom hargs |
-      ????????? he hm hdom hargs |
-      ???? hsub h hi | ?????? hin hr h hi | ????? hin hr h hi |
-      ????? hin hr h hi | ????? hin hr h hi | ????? hin hr h hi |
-      ????? hcond hthn hi1 hels hi2 | ???? he hnotthis |
-      ???? hrecv hrhs hnotthis | ????? he hargs hnotthis
+    induction 1 as [ ? lty | ?????? h1 hi1 h2 hi2 | ????? he |
+      ?????? he h1 hi1 h2 hi2 | ??????? he hf | ????????? he hf |
+      ??????? he hf hr | ????????? he hf hr | ??????? ht hok hf hdom hargs |
+      ?????????? he hm hdom hargs |
+      ????? hsub h hi | ??????? hin hr h hi | ?????? hin hr h hi |
+      ?????? hin hr h hi | ?????? hin hr h hi | ?????? hin hr h hi |
+      ?????? hcond hthn hi1 hels hi2 | ????? he hnotthis |
+      ????? hrecv hrhs hnotthis | ?????? he hargs hnotthis
       ] => Γ' hincl.
     + by constructor.
     + econstructor; by eauto.
@@ -660,20 +660,20 @@ Section Typing.
       - by destruct recv.
   Qed.
 
-  Lemma cmd_has_ty_constraint_elim_ G lty cmd rty:
-    cmd_has_ty G lty cmd rty →
+  Lemma cmd_has_ty_constraint_elim_ G kd lty cmd rty:
+    cmd_has_ty G kd lty cmd rty →
     ∀ Γ Γ', G = Γ ++ Γ' →
-    (∀ i c, Γ' !! i = Some c → Γ ⊢ c.1 <: c.2) →
-    cmd_has_ty Γ lty cmd rty.
+    (∀ i c, Γ' !! i = Some c → Γ ⊢ c.1 <D: c.2) →
+    cmd_has_ty Γ kd lty cmd rty.
   Proof.
-    induction 1 as [ lty | ????? h1 hi1 h2 hi2 | ???? he |
-      ????? he h1 hi1 h2 hi2 | ?????? he hf | ???????? he hf |
-      ?????? he hf hr | ???????? he hf hr | ?????? ht hok hf hdom hargs |
-      ????????? he hm hdom hargs |
-      ???? hsub h hi | ?????? hin hr h hi | ????? hin hr h hi |
-      ????? hin hr h hi | ????? hin hr h hi | ????? hin hr h hi |
-      ????? hcond hthn hi1 hels hi2 | ???? he hnotthis |
-      ???? hrecv hrhs hnotthis | ????? he hargs hnotthis
+    induction 1 as [ ? lty | ?????? h1 hi1 h2 hi2 | ????? he |
+      ?????? he h1 hi1 h2 hi2 | ??????? he hf | ????????? he hf |
+      ??????? he hf hr | ????????? he hf hr | ??????? ht hok hf hdom hargs |
+      ?????????? he hm hdom hargs |
+      ????? hsub h hi | ??????? hin hr h hi | ?????? hin hr h hi |
+      ?????? hin hr h hi | ?????? hin hr h hi | ?????? hin hr h hi |
+      ?????? hcond hthn hi1 hels hi2 | ????? he hnotthis |
+      ????? hrecv hrhs hnotthis | ?????? he hargs hnotthis
       ] => Γ Γ' heq hΓ; subst.
     - by econstructor.
     - econstructor; by eauto.
@@ -700,7 +700,7 @@ Section Typing.
       + move => ?????.
         eapply expr_has_ty_constraint_elim; by eauto.
     - econstructor => //.
-      + by eapply lty_sub_constraint_elim.
+      + eapply lty_sub_constraint_elim => //.
       + by eauto.
     - eapply TagCheckTy => //.
       + by eapply lty_sub_constraint_elim.
@@ -732,30 +732,30 @@ Section Typing.
         by eapply hargs.
   Qed.
 
-  Lemma cmd_has_ty_constraint_elim Γ Γ' lty cmd rty:
-    cmd_has_ty (Γ ++ Γ') lty cmd rty →
-    (∀ i c, Γ' !! i = Some c → Γ ⊢ c.1 <: c.2) →
-    cmd_has_ty Γ lty cmd rty.
+  Lemma cmd_has_ty_constraint_elim Γ Γ' kd lty cmd rty:
+    cmd_has_ty (Γ ++ Γ') kd lty cmd rty →
+    (∀ i c, Γ' !! i = Some c → Γ ⊢ c.1 <D: c.2) →
+    cmd_has_ty Γ kd lty cmd rty.
   Proof. intros; by eapply cmd_has_ty_constraint_elim_. Qed.
 
-  Lemma cmd_has_ty_wf Γ lty cmd lty' :
+  Lemma cmd_has_ty_wf Γ kd lty cmd lty' :
     map_Forall (λ _ : string, wf_cdef_parent Δ) Δ →
     map_Forall (λ _ : string, wf_cdef_fields_wf) Δ →
     map_Forall (λ _ : string, wf_cdef_methods_wf) Δ →
     Forall wf_constraint Γ →
     wf_lty lty →
-    cmd_has_ty Γ lty cmd lty' →
+    cmd_has_ty Γ kd lty cmd lty' →
     wf_lty lty'.
   Proof.
     move => hp hfields hmethods hΓ [hthis hwf].
-    induction 1 as [ lty | ????? h1 hi1 h2 hi2 | ???? he |
-      ????? he h1 hi1 h2 hi2 | ?????? he hf | ???????? he hf |
-      ?????? he hf hr | ???????? he hf hr | ?????? ht hok hf hdom hargs |
-      ????????? he hm hdom hargs |
-      ???? hsub h hi | ?????? hin hr h hi | ????? hin hr h hi |
-      ????? hin hr h hi | ????? hin hr h hi | ????? hin hr h hi |
-      ????? hcond hthn hi1 hels hi2 | ???? he hnotthis |
-      ???? hrecv hrhs hnotthis | ????? he hargs hnotthis
+    induction 1 as [ | ?????? h1 hi1 h2 hi2 | ????? he |
+      ?????? he h1 hi1 h2 hi2 | ??????? he hf | ????????? he hf |
+      ??????? he hf hr | ????????? he hf hr | ??????? ht hok hf hdom hargs |
+      ?????????? he hm hdom hargs |
+      ????? hsub h hi | ??????? hin hr h hi | ?????? hin hr h hi |
+      ?????? hin hr h hi | ?????? hin hr h hi | ?????? hin hr h hi |
+      ?????? hcond hthn hi1 hels hi2 | ????? he hnotthis |
+      ????? hrecv hrhs hnotthis | ?????? he hargs hnotthis
       ] => //=; try (by eauto).
     - apply hi2.
       + by apply hi1.
@@ -843,8 +843,7 @@ Section Typing.
     - by apply insert_wf_lty.
   Qed.
 
-
-  Lemma cmd_has_ty_subst Γ' Γ σ lty cmd lty':
+  Lemma cmd_has_ty_subst Γ' Γ kd σ lty cmd lty':
     map_Forall (λ _ : string, wf_cdef_parent Δ) Δ →
     map_Forall (λ _ : string, wf_cdef_fields_wf) Δ →
     map_Forall (λ _ : string, wf_cdef_methods_wf) Δ →
@@ -855,23 +854,23 @@ Section Typing.
     wf_lty lty →
     Forall wf_ty σ →
     Forall (ok_ty Γ') σ →
-    cmd_has_ty Γ lty cmd lty' →
-    cmd_has_ty (Γ' ++ (subst_constraints σ Γ)) (subst_lty σ lty) (subst_cmd σ cmd) (subst_lty σ lty').
+    cmd_has_ty Γ kd lty cmd lty' →
+    cmd_has_ty (Γ' ++ (subst_constraints σ Γ)) kd (subst_lty σ lty) (subst_cmd σ cmd) (subst_lty σ lty').
   Proof.
     move => hp hfields hmethods hfb hmb hcb hΓ hwf0 hwf1 hwf2.
-    induction 1 as [ lty | ????? h1 hi1 h2 hi2 | ???? he |
-      ????? he h1 hi1 h2 hi2 | ?????? he hf | ???????? he hf |
-      ?????? he hf hr | ???????? he hf hr | ?????? hwf hok hf hdom hargs |
-      ????????? he hm hdom hargs |
-      ???? hsub h hi | ?????? hin hr h hi | ????? hin hr h hi |
-      ????? hin hr h hi | ????? hin hr h hi | ????? hin hr h hi |
-      ????? hcond hthn hi1 hels hi2 | ???? he hnotthis |
-      ???? hrecv hrhs hnotthis | ????? he hargs hnotthis
+    induction 1 as [ | ?????? h1 hi1 h2 hi2 | ????? he |
+      ?????? he h1 hi1 h2 hi2 | ??????? he hf | ????????? he hf |
+      ??????? he hf hr | ????????? he hf hr | ??????? hwf hok hf hdom hargs |
+      ?????????? he hm hdom hargs |
+      ????? hsub h hi | ??????? hin hr h hi | ?????? hin hr h hi |
+      ?????? hin hr h hi | ?????? hin hr h hi | ?????? hin hr h hi |
+      ?????? hcond hthn hi1 hels hi2 | ????? he hnotthis |
+      ????? hrecv hrhs hnotthis | ?????? he hargs hnotthis
       ] => //=.
     - by constructor.
     - econstructor.
       + by eapply hi1.
-      + eapply hi2.
+      + eapply hi2 => //.
         by apply cmd_has_ty_wf in h1.
     - rewrite /subst_lty fmap_insert.
       eapply LetTy.
@@ -880,8 +879,7 @@ Section Typing.
       + change BoolT with (subst_ty σ BoolT).
         by eapply expr_has_ty_subst.
       + by apply hi1.
-      + apply hi2.
-        by apply cmd_has_ty_wf in h1.
+      + by apply hi2.
     - destruct lty as [[this σt] lty].
       destruct hwf0 as [hthis hwf].
       simpl in *.
@@ -1000,7 +998,7 @@ Section Typing.
       + apply lty_sub_weaken with (subst_constraints σ Γ); last by set_solver.
         by apply lty_sub_subst.
       + rewrite /subst_lty fmap_insert /= in hi.
-        apply hi.
+        apply hi => //.
         destruct lty as [[lt lσ] lty].
         split.
         * rewrite /this_type /=.
@@ -1013,7 +1011,7 @@ Section Typing.
       + apply lty_sub_weaken with (subst_constraints σ Γ); last by set_solver.
         by apply lty_sub_subst.
       + rewrite /subst_lty fmap_insert /= in hi.
-        apply hi.
+        apply hi => //.
         destruct lty as [[lt lσ] lty].
         split.
         * rewrite /this_type /=.
@@ -1026,7 +1024,7 @@ Section Typing.
       + apply lty_sub_weaken with (subst_constraints σ Γ); last by set_solver.
         by apply lty_sub_subst.
       + rewrite /subst_lty fmap_insert /= in hi.
-        apply hi.
+        apply hi => //.
         destruct lty as [[lt lσ] lty].
         split.
         * rewrite /this_type /=.
@@ -1039,7 +1037,7 @@ Section Typing.
       + apply lty_sub_weaken with (subst_constraints σ Γ); last by set_solver.
         by apply lty_sub_subst.
       + rewrite /subst_lty fmap_insert /= in hi.
-        apply hi.
+        apply hi => //.
         destruct lty as [[lt lσ] lty].
         split.
         * rewrite /this_type /=.
@@ -1052,7 +1050,7 @@ Section Typing.
       + apply lty_sub_weaken with (subst_constraints σ Γ); last by set_solver.
         by apply lty_sub_subst.
       + rewrite /subst_lty fmap_insert /= in hi.
-        apply hi.
+        apply hi => //.
         destruct lty as [[lt lσ] lty].
         split.
         * rewrite /this_type /=.
@@ -1064,8 +1062,7 @@ Section Typing.
       + change DynamicT with (subst_ty σ DynamicT).
         by eapply expr_has_ty_subst.
       + by apply hi1.
-      + apply hi2.
-        by apply cmd_has_ty_wf in hthn.
+      + by apply hi2.
     - replace (subst_lty σ (<[lhs:=DynamicT]> lty)) with
              (<[lhs := DynamicT]>(subst_lty σ lty)); last first.
       { rewrite /subst_lty /= /insert /local_tys_insert /=.
@@ -1107,10 +1104,10 @@ Section Typing.
   Definition wf_mdef_ty Γ tag σ mdef :=
     ∃ rty,
     wf_lty rty ∧
-    cmd_has_ty Γ
+    cmd_has_ty Γ Plain
       {| type_of_this := (tag, σ); ctxt := subst_ty σ <$> mdef.(methodargs) |}
       mdef.(methodbody) rty ∧
-    expr_has_ty Γ rty mdef.(methodret) (subst_ty σ mdef.(methodrettype))
+    expr_has_ty Γ rty Plain mdef.(methodret) (subst_ty σ mdef.(methodrettype))
   .
 
   Definition cdef_wf_mdef_ty cname cdef :=
@@ -1124,10 +1121,10 @@ Section Typing.
   Definition wf_mdef_dyn_ty Γ tag σ mdef :=
     ∃ rty,
     wf_lty rty ∧
-    cmd_has_ty Γ
+    cmd_has_ty Γ Aware
       {| type_of_this := (tag, σ); ctxt := to_dyn <$> mdef.(methodargs) |}
       mdef.(methodbody) rty ∧
-    expr_has_ty Γ rty mdef.(methodret) (to_dyn mdef.(methodrettype))
+    expr_has_ty Γ rty Aware mdef.(methodret) (to_dyn mdef.(methodrettype))
   .
 
   Definition wf_cdef_methods_dyn_wf cname cdef :=
@@ -1149,7 +1146,7 @@ Section Typing.
     match vfty.1 with
     | (Private, _) => True
     | (Public, fty) =>
-        Σc ⊢ fty <: DynamicT ∧ Σc ⊢ DynamicT <: fty
+        Σc ⊢ fty <D: DynamicT ∧ Σc ⊢ DynamicT <D: fty
     end.
 
   Definition wf_cdef_fields_dyn_wf cname cdef :=
@@ -1256,7 +1253,7 @@ Section MethodTyping.
 
   (* Helping the inference with this notation that hides Δ *)
   Local Notation "Γ ⊢ s <: t" := (@subtype _ Γ Plain s t) (at level 70, s at next level, no associativity).
-  Local Notation "Γ ⊢ lty <:< rty" := (@lty_sub _ Γ lty rty) (lty at next level, at level 70, no associativity).
+  Local Notation "Γ ⊢ s <D: t" := (@subtype _ Γ Aware s t) (at level 70, s at next level, no associativity).
 
   (* Let's consider that class C0 has/inherits a method m from class C1
    * where it is declared. Then m is correctly typed in C0 for any valid
@@ -1268,9 +1265,9 @@ Section MethodTyping.
     def.(classmethods) !! m = Some mdef →
     wf_ty (ClassT C σ) → ok_ty Σc (ClassT C σ) →
     ∃ rty, wf_lty rty ∧
-      cmd_has_ty Σc {| type_of_this := (C, σ); ctxt := subst_ty σ <$> mdef.(methodargs) |}
+      cmd_has_ty Σc Plain {| type_of_this := (C, σ); ctxt := subst_ty σ <$> mdef.(methodargs) |}
                 (subst_cmd σ mdef.(methodbody)) rty ∧
-      expr_has_ty Σc rty (subst_expr σ mdef.(methodret)) (subst_ty σ mdef.(methodrettype)).
+      expr_has_ty Σc rty Plain (subst_expr σ mdef.(methodret)) (subst_ty σ mdef.(methodrettype)).
   Proof.
     move => hΔ hdef hmdef hwf hok.
     destruct hΔ.
@@ -1279,11 +1276,11 @@ Section MethodTyping.
     assert (hokσ : Forall (ok_ty Σc) σ) by (by apply ok_ty_class_inv in hok).
     (* Let's use the general substitution lemma to make the instantiation *)
     assert (hgen : ∃ rty, wf_lty rty ∧
-      cmd_has_ty (Σc ++ subst_constraints σ def.(constraints))
+      cmd_has_ty (Σc ++ subst_constraints σ def.(constraints)) Plain
                  (subst_lty σ {| type_of_this := (C, gen_targs (length def.(generics))); ctxt := mdef.(methodargs) |})
                  (subst_cmd σ mdef.(methodbody)) rty ∧
       expr_has_ty (Σc ++ subst_constraints σ def.(constraints))
-                  rty (subst_expr σ mdef.(methodret)) (subst_ty σ mdef.(methodrettype))).
+                  rty Plain (subst_expr σ mdef.(methodret)) (subst_ty σ mdef.(methodrettype))).
     { assert (hd := hdef).
       assert (hm := hmdef).
       apply wf_mdefs0 in hd.
@@ -1322,7 +1319,7 @@ Section MethodTyping.
      *)
     assert (hconstraints: ∀ i c,
       (subst_constraints σ (constraints def)) !! i = Some c →
-      Σc ⊢ c.1 <: c.2).
+      Σc ⊢ c.1 <D: c.2).
     { move => i c hin.
       apply list_lookup_fmap_inv in hin as [c' [-> hin]].
       inv hok; simplify_eq.
