theories/examples.v
@@ -341,7 +341,7 @@ Definition final_lty lty : local_tys :=
   (<["$robox" := ClassT "ROBox" [IntT]]> lty)))).
 
 Lemma Main_ty lty :
-  cmd_has_ty [] lty ProgramBody (final_lty lty).
+  cmd_has_ty [] Plain lty ProgramBody (final_lty lty).
 Proof.
   rewrite /final_lty /ProgramBody.
   eapply SeqTy.
@@ -1348,7 +1348,7 @@ Qed.
  *)
 Theorem int_adequacy cmd st lty n:
   cmd_eval (main_le, main_heap "Main") cmd st n →
-  cmd_has_ty [] (main_lty "Main") cmd lty →
+  cmd_has_ty [] Plain (main_lty "Main") cmd lty →
   ∀ v, lty.(ctxt) !! v = Some IntT →
   ∃ z, st.1.(lenv) !! v = Some (IntV z).
 Proof.
@@ -1373,7 +1373,7 @@ Proof.
   { iIntros (? ? h).
     by rewrite lookup_nil in h.
   }
-  iDestruct ((cmd_adequacy [] [] _ _ _ wf wfinit wfΣc ht _ _ _ he) with "wfΣi Σcoherency Hmain") as "H" => /=.
+  iDestruct ((cmd_adequacy [] _ [] _ _ _ wf wfinit wfΣc ht _ _ _ he) with "wfΣi Σcoherency Hmain") as "H" => /=.
   iRevert "H".
   iApply updN_mono.
   iIntros "[Hh [Hthis Hl]]".
@@ -1386,7 +1386,7 @@ Qed.
 
 Theorem class_adequacy cmd st lty n:
   cmd_eval (main_le, main_heap "Main") cmd st n →
-  cmd_has_ty [] (main_lty "Main") cmd lty →
+  cmd_has_ty [] Plain (main_lty "Main") cmd lty →
   ∀ v T σ, lty.(ctxt) !! v = Some (ClassT T σ) →
   ∃ l Tdyn vs, st.1.(lenv) !! v = Some (LocV l) ∧
           st.2 !! l = Some (Tdyn, vs) ∧
@@ -1413,7 +1413,7 @@ Proof.
   { iIntros (? ? h).
     by rewrite lookup_nil in h.
   }
-  iDestruct ((cmd_adequacy [] [] _ _ _ wf wfinit wfΣc ht _ _ _ he) with "wfΣi Σcoherency Hmain") as "H" => /=.
+  iDestruct ((cmd_adequacy [] _ [] _ _ _ wf wfinit wfΣc ht _ _ _ he) with "wfΣi Σcoherency Hmain") as "H" => /=.
   iRevert "H".
   iApply updN_mono.
   iIntros "[Hh [_ Hl]]".
